specs/ecdsap256sha2/Spec.P256.MontgomeryMultiplication.fst
@@ -72,7 +72,7 @@ let multiplicationInDomainNat #k #l a b =
   lemma_twice_brackets k (pow2 256) 1 l (pow2 256) 1 (modp_inv2 (pow2 256));
   assert_norm (pow2 256 * modp_inv2 (pow2 256) % prime == 1);
   modulo_distributivity_mult_last_two k (pow2 256) l (pow2 256) (modp_inv2 (pow2 256)) prime;
-  lemma_mul_ass3 k (pow2 256) l
+  lemma_mul_associativity_3 k (pow2 256) l
 
 let additionInDomain a b =
   let k = fromDomain_ a in
